\section*{4. The \textsc{nand} operation}

Define $x \uparrow y \;=\; \lnot(x \land y)$.

\subsection*{(a) Truth table}
\[
\begin{array}{c c c c}
x & y & x \land y & x \uparrow y=\lnot(x\land y)\\ \hline
\mathrm{T} & \mathrm{T} & \mathrm{T} & \mathrm{F}\\
\mathrm{T} & \mathrm{F} & \mathrm{F} & \mathrm{T}\\
\mathrm{F} & \mathrm{T} & \mathrm{F} & \mathrm{T}\\
\mathrm{F} & \mathrm{F} & \mathrm{F} & \mathrm{T}
\end{array}
\]

\subsection*{(b) Commutativity and associativity}
\textbf{Commutative.} Since $\land$ is commutative and negation preserves equality,
\[
x \uparrow y \;=\; \lnot(x\land y) \;=\; \lnot(y\land x) \;=\; y \uparrow x.
\]

\noindent
\textbf{Not associative.} Using $x=\mathrm{T},\,y=\mathrm{T},\,z=\mathrm{F}$:
\[
(x\uparrow y)\uparrow z \;=\; (\mathrm{T}\uparrow \mathrm{T})\uparrow \mathrm{F}
= \mathrm{F}\uparrow \mathrm{F} = \mathrm{T},
\]
\[
x\uparrow (y\uparrow z) \;=\; \mathrm{T}\uparrow (\mathrm{T}\uparrow \mathrm{F})
= \mathrm{T}\uparrow \mathrm{T} = \mathrm{F}.
\]
The results differ, so $\uparrow$ is \emph{not} associative.

\subsection*{(c) Expressing $\boldsymbol{x\land y}$ and $\boldsymbol{\lnot x}$ using only $\boldsymbol{\uparrow}$}
Using the definition,
\[
\lnot x \;\equiv\; x \uparrow x
\qquad\text{since}\qquad x\uparrow x=\lnot(x\land x)=\lnot x,
\]
and
\[
x\land y \;\equiv\; (x\uparrow y)\uparrow (x\uparrow y)
\qquad\text{since}\qquad (x\uparrow y)\uparrow (x\uparrow y)
= \lnot\bigl(\lnot(x\land y)\bigr)=x\land y.
\]

\paragraph{Functional completeness of $\uparrow$.}
Problem 3 shows that every binary Boolean operation is expressible using only $\{\land,\lnot\}$.
Because both $\land$ and $\lnot$ are definable using only $\uparrow$, it follows that $\uparrow$
alone is functionally complete.
