\section*{3. Writing $\boldsymbol{x\lor y}$ using only $\boldsymbol{\land}$ and $\boldsymbol{\lnot}$}
By De Morgan's law,
\[
x\lor y \;\equiv\; \lnot(\lnot x \land \lnot y).
\]
For completeness, the truth-table verification:

\[
\begin{array}{c c c c}
x & y & x\lor y & \lnot(\lnot x \land \lnot y)\\ \hline
\mathrm{T} & \mathrm{T} & \mathrm{T} & \lnot(\mathrm{F}\land \mathrm{F})=\lnot\mathrm{F}=\mathrm{T}\\
\mathrm{T} & \mathrm{F} & \mathrm{T} & \lnot(\mathrm{F}\land \mathrm{T})=\lnot\mathrm{F}=\mathrm{T}\\
\mathrm{F} & \mathrm{T} & \mathrm{T} & \lnot(\mathrm{T}\land \mathrm{F})=\lnot\mathrm{F}=\mathrm{T}\\
\mathrm{F} & \mathrm{F} & \mathrm{F} & \lnot(\mathrm{T}\land \mathrm{T})=\lnot\mathrm{T}=\mathrm{F}
\end{array}
\]

\paragraph{Conclusion.}
From Problem 2, any binary Boolean operation is expressible using $\{\land,\lor,\lnot\}$.
Replacing every occurrence of $\lor$ in such an expression by $\lnot(\lnot n \land \lnot j)$
yields an equivalent expression containing only $\{\land,\lnot\}$.
Hence every binary Boolean operation is expressible using just $\{\land,\lnot\}$.
