\section*{1. Exclusive or (XOR)}

The Boolean operation \emph{exclusive or} (XOR), written $x \xor y$, is defined by:
\[
\begin{array}{c c | c}
x & y & x \xor y\\ \hline
\mathrm{T} & \mathrm{T} & \mathrm{F}\\
\mathrm{T} & \mathrm{F} & \mathrm{T}\\
\mathrm{F} & \mathrm{T} & \mathrm{T}\\
\mathrm{F} & \mathrm{F} & \mathrm{F}
\end{array}
\]

\subsection*{(a) Commutativity and associativity}

\paragraph{Commutativity.}
From the table above, $x \xor y$ and $y \xor x$ have identical outputs for all four
assignments of $(x,y)$, hence $x \xor y \equiv y \xor x$.

\medskip
\paragraph{Associativity.}
We verify that $(x \xor y) \xor z \equiv x \xor (y \xor z)$ by a truth table on three variables.

\[
\begin{array}{c c c | c | c | c | c}
x & y & z & x \oplus y & y \oplus z & (x \oplus y) \oplus z & x \oplus (y \oplus z)\\ \hline
\mathrm{T} & \mathrm{T} & \mathrm{T} & \mathrm{F} & \mathrm{F} & \mathrm{T} & \mathrm{T}\\
\mathrm{T} & \mathrm{T} & \mathrm{F} & \mathrm{F} & \mathrm{T} & \mathrm{F} & \mathrm{F}\\
\mathrm{T} & \mathrm{F} & \mathrm{T} & \mathrm{T} & \mathrm{T} & \mathrm{F} & \mathrm{F}\\
\mathrm{T} & \mathrm{F} & \mathrm{F} & \mathrm{T} & \mathrm{F} & \mathrm{T} & \mathrm{T}\\
\mathrm{F} & \mathrm{T} & \mathrm{T} & \mathrm{T} & \mathrm{F} & \mathrm{F} & \mathrm{F}\\
\mathrm{F} & \mathrm{T} & \mathrm{F} & \mathrm{T} & \mathrm{T} & \mathrm{T} & \mathrm{T}\\
\mathrm{F} & \mathrm{F} & \mathrm{T} & \mathrm{F} & \mathrm{T} & \mathrm{T} & \mathrm{T}\\
\mathrm{F} & \mathrm{F} & \mathrm{F} & \mathrm{F} & \mathrm{F} & \mathrm{F} & \mathrm{F}
\end{array}
\]

Both last columns agree in every row, so $(x \xor y)\xor z \equiv x \xor (y \xor z)$.
Therefore $\xor$ is associative.

\subsection*{(b) Standard connective form}

We show that
\[
x \xor y \;\equiv\; (x \land \lnot y) \;\lor\; (\lnot x \land y).
\]
First recall the equivalent description of XOR as ``exactly one is true'':
\[
x \xor y \equiv (x \lor y)\land \lnot(x \land y).
\]
Applying De~Morgan and distributivity,
\[
\begin{aligned}
(x \lor y)\land \lnot(x \land y)
&\equiv (x \lor y)\land (\lnot x \lor \lnot y) \\
&\equiv \bigl(x\land(\lnot x \lor \lnot y)\bigr)\;\lor\;\bigl(y\land(\lnot x \lor \lnot y)\bigr) \\
&\equiv (x\land\lnot x)\;\lor\;(x\land\lnot y)\;\lor\;(\lnot x\land y)\;\lor\;(y\land\lnot y) \\
&\equiv (x\land\lnot y)\;\lor\;(\lnot x\land y),
\end{aligned}
\]
since $x\land\lnot x \equiv \bot$ and $y\land\lnot y \equiv \bot$.
This completes the proof.
